Definitions in DeltaCorrectness, and equivalence of correctness game between schemes (required some adjustments in prelims as well).

Security/SaberRqDeltaCorrectness.ec
@@ -9,14 +9,13 @@ require import AllCore Distr ZModP IntDiv StdOrder List.
 (* --- Local --- *)
 require import SaberRqPreliminaries.
 (*---*) import Saber_PKE.
-(*---*) import Mat_Rp Mat_Rq.
 (*---*) import Zp Rp Rp.ComRing Rp.BasePoly.
 (*---*) import Zq Rq Rq.ComRing Rq.BasePoly. 
 (*---*) import Zppq Rppq Rppq.ComRing Rppq.BasePoly.
 (*---*) import Z2t R2t R2t.ComRing R2t.BasePoly.
 (*---*) import Z2 R2 R2.ComRing R2.BasePoly.
 
-(*
+
 (* ----------------------------------- *)
 (*  Adversary Prototypes               *)
 (* ----------------------------------- *)
@@ -26,10 +25,10 @@ module type Adv_Cor = {
 }.
 
 (* ----------------------------------- *)
-(*  Saber PKE Correctness Game         *)
+(*  Correctness Game                   *)
 (* ----------------------------------- *)
 
-module Saber_PKE_Correctness (A : Adv_Cor) = {
+module Correctness_Game (S : Scheme, A : Adv_Cor) = {
    proc main() : bool = {
       var m: plaintext;
       var m': plaintext option;
@@ -37,444 +36,115 @@ module Saber_PKE_Correctness (A : Adv_Cor) = {
       var pk: pkey;
       var sk: skey;
       
-      (pk, sk) <@ Saber_PKE_Scheme.kg();
+      (pk, sk) <@ S.kg();
       m <@ A.choose(pk, sk);
-      c <@ Saber_PKE_Scheme.enc(pk, m);
-      m' <@ Saber_PKE_Scheme.dec(sk, c);
+      c <@ S.enc(pk, m);
+      m' <@ S.dec(sk, c);
 
       return (Some m = m');
    }
 }.
 
-(* ----------------------------------- *)
-(* All Rq                              *)
-(* ----------------------------------- *)
-
-lemma upscale_DM (ea eb : int) : morphism_2 (fun x => upscale x ea eb) Int.(+) Int.(+).
-proof. by move => x y; rewrite /upscale /shl mulrDl. qed.
-
-lemma scale_DM (x y ea eb : int) : 
-  2 ^ (ea - eb) %| x \/  2 ^ (ea - eb) %| y => 
-  downscale (x + y) ea eb = downscale x ea eb + downscale y ea eb.
-proof. by case; rewrite /scale /shr; [apply divzDl | apply divzDr]. qed.
-
-lemma scaleZp2Z2t_DM (z1 z2 : Zp) : 
-  2 ^ (ep - (et + 1)) %| Zp.asint z1 \/  2 ^ (ep - (et + 1)) %| Zp.asint z2 => 
-  scaleZp2Z2t (z1 + z2) = scaleZp2Z2t z1 + scaleZp2Z2t z2.
-proof. 
-case => [divz1 | divz2]; rewrite /scaleZp2Z2t -inzmodD -scale_DM ?(divz1, divz2) //;
-    rewrite addE /p /downscale /shr /inzmod /t -exprS 1:ge0_et modz_pow2_div;
-    1, 2, 4, 5: smt(Zp.ge0_asint geet2_ep ge0_et); congr; rewrite modz_dvd_pow; smt(ge0_et).
+(* Equivalence of Correctness Games with Regular and Alternative PKE Description *)
+lemma eq_Correctness_Game_Reg_Alt (A <: Adv_Cor) :
+  equiv[Correctness_Game(Saber_PKE_Scheme, A).main ~ Correctness_Game(Saber_PKE_Scheme_Alt, A).main 
+        : ={glob A} ==> ={res}].
+proof.
+proc.
+call eq_dec; call eq_enc; call (_ : true); call eq_kg.
+by auto.
 qed.
 
-lemma scaleZq2Z2t_DM (z1 z2 : Zq) : 
-  2 ^ (eq - (et + 1)) %| Zq.asint z1 \/  2 ^ (eq - (et + 1)) %| Zq.asint z2 => 
-  scaleZq2Z2t (z1 + z2) = scaleZq2Z2t z1 + scaleZq2Z2t z2.
-proof. 
-case => [divz1 | divz2]; rewrite /scaleZq2Z2t -inzmodD -scale_DM ?(divz1, divz2) //;
-    rewrite addE /q /downscale /shr /inzmod /t -exprS 1:ge0_et modz_pow2_div;
-    1, 2, 4, 5: smt(Zq.ge0_asint geet2_ep geep1_eq ge0_et); congr; rewrite modz_dvd_pow; smt(ge0_et).
-qed.
+(* ----------------------------------- *)
+(*  Error                              *)
+(* ----------------------------------- *)
+
+clone Matrix as Mat_int with
+  type R    <- int,
+    op size <- n.
+
+type int_vec = Mat_int.vector.
+
+(*---*) import Mat_Rp Mat_Rq Mat_int.
+
+abbrev ( - ) (pv1 pv2 : Rq_vec) = pv1 + (- pv2).
+  
+op errorZq (z1 z2 : Zq) : Zq = z1 - z2.
+op errorRq (p1 p2 : Rq) : Rq = p1 - p2.
+op errorRqv (pv1 pv2 : Rq_vec) : Rq_vec = pv1 - pv2.
+
+op interrorZq (z1 z2 : Zq) : int = `| Zq.asint z1 - Zq.asint z2 |.
+op interrorRq (p1 p2 : Rq) : int_vec = offunv (fun (i : int) => interrorZq p1.[i] p2.[i]).
+op interrorRqv (pv1 pv2 : Rq_vec) : int_vec list = mkseq (fun (i : int) => interrorRq pv1.[i] pv2.[i]) l.
+
 
 (*
-scaleRp2R2t
-  (dotp (pk_decode pk{2}).`2 (Rqv2Rpv s'L) + Rq2Rp h1 +
-   shl_enc (m_decode m{2}) (ep - 1)) 
-=
-scaleRq2R2t
-  (dotp (scaleRpv2Rqv (pk_decode pk{2}).`2) s'L + scaleRq h1 (eq - ep) +
-   scaleR22Rq (m_decode m{2}))
+axiom errorRq_def (p1 p2 : Rq) : 
+  exists (i : int), 
+  (0 <= i < n => 
+  errorRq p1 p2 = errorZq p1.[i] p2.[i] /\ 
+  forall (j : int), 0 <= j < n => max (errorRq p1 p2) (errorZq p1.[j] p2.[j]) = errorRq p1 p2).
 *)
-lemma scaleRp2R2t_DM (p1 p2 : Rp) : 
-  ((forall (i : int), 0 <= i < n =>  2 ^ (ep - (et + 1)) %| Zp.asint p1.[i]) \/  
-  (forall (i : int), 0 <= i < n =>  2 ^ (ep - (et + 1)) %| Zp.asint p2.[i])) =>
-  scaleRp2R2t (p1 + p2) = scaleRp2R2t p1 + scaleRp2R2t p2.
-proof.
-case => [divz1 | divz2]; rewrite /scaleRp2R2t eq_sym -BigR2t.XnD1CA.big_split /=;
-    rewrite !BigR2t.XnD1CA.big_seq &(BigR2t.XnD1CA.eq_bigr) /= => i /mem_range rng_i;
-    rewrite -scaleDl eq_sym rcoeffD scaleZp2Z2t_DM ?(divz1, divz2) //.
-qed.
 
-lemma scaleRq2R2t_DM (p1 p2 : Rq) : 
-  ((forall (i : int), 0 <= i < n =>  2 ^ (eq - (et + 1)) %| Zq.asint p1.[i]) \/  
-  (forall (i : int), 0 <= i < n =>  2 ^ (eq - (et + 1)) %| Zq.asint p2.[i])) =>
-  scaleRq2R2t (p1 + p2) = scaleRq2R2t p1 + scaleRq2R2t p2.
-proof.
-case => [divz1 | divz2]; rewrite /scaleRq2R2t eq_sym -BigR2t.XnD1CA.big_split /=;
-    rewrite !BigR2t.XnD1CA.big_seq &(BigR2t.XnD1CA.eq_bigr) /= => i /mem_range rng_i;
-    rewrite -scaleDl eq_sym rcoeffD scaleZq2Z2t_DM ?(divz1, divz2) //.
-qed.
+op error_bq0 (s bq : Rq_vec) (_A : Rq_mat) : Rq_vec = errorRqv bq (_A *^ s).
+op error_bq0' (s' bq' : Rq_vec) (_A : Rq_mat) : Rq_vec = errorRqv bq' ((trmx _A) *^ s').
+op error_cmq0 (cmq v' m_dec: Rq) : Rq = errorRq cmq (v' + m_dec).
 
-lemma scaleZp2Zq0 : scaleZp2Zq Zp.zero = Zq.zero.
-proof. by rewrite /scaleZp2Zq /upscale /shl zeroE. qed.
+op interror_bq (s bq : Rq_vec) (_A : Rq_mat) : int_vec list = interrorRqv bq (_A *^ s).
+op interror_bq' (s' bq' : Rq_vec) (_A : Rq_mat) : int_vec list = interrorRqv bq' ((trmx _A) *^ s').
+op interror_cmq (cmq v' m_dec: Rq) : int_vec = interrorRq cmq (v' + m_dec).
 
-lemma scaleZp2Zq_DM (z1 z2 : Zp) : scaleZp2Zq (z1 + z2) = scaleZp2Zq z1 + scaleZp2Zq z2.
-proof.
-rewrite /scaleZp2Zq -inzmodD /upscale /shl -mulrDl addE -eq_inzmod /p /q modz_pow2_mul //.
-+ smt(ge2_ep geep1_eq).
-qed.
+op error_bq (_A : Rq_mat) (s : Rq_vec) : Rq_vec = 
+  errorRqv (scaleRpv2Rqv (scaleRqv2Rpv (_A *^ s + h))) (_A *^ s).
+op error_bq' (_A : Rq_mat) (s': Rq_vec) : Rq_vec = 
+  errorRqv (scaleRpv2Rqv (scaleRqv2Rpv ((trmx _A) *^ s' + h))) ((trmx _A) *^ s').
 
-lemma scaleZp2Zq_BM (z1 z2 : Zp) : scaleZp2Zq (z1 - z2) = scaleZp2Zq z1 - scaleZp2Zq z2.
-proof.
-rewrite /scaleZp2Zq -inzmodB /upscale /shl addE oppE -mulrBl -eq_inzmod /p /q.
-rewrite modzDmr modz_pow2_mul //.
-+ smt(ge2_ep geep1_eq).
-qed.
+op v_expression (_A : Rq_mat) (s s': Rq_vec) : Rq =
+  let bq' = ((trmx _A) *^ s') + (error_bq' _A s') in 
+  (dotp bq' s) + (upscaleRq h1 (eq - ep)).
 
-lemma scaleZp2Zq_MA (z1 z2 : Zp) : scaleZp2Zq (z1 * z2) = scaleZp2Zq z1 * Zp2Zq z2.
-proof.
-rewrite /scaleZp2Zq /Zp2Zq -inzmodM /upscale /shl mulrAC mulE -eq_inzmod /p /q modz_pow2_mul //.
-+ smt(ge2_ep geep1_eq).
-qed.
+op v'_expression (_A : Rq_mat) (s s': Rq_vec) : Rq =
+  let bq = (_A *^ s) + (error_bq _A s) in
+  (dotp bq s') + (upscaleRq h1 (eq - ep)).
+
+op error_cmq (_A : Rq_mat) (s s': Rq_vec) (m : R2) : Rq =
+  let v' = v'_expression _A s s' in
+  errorRq (scaleR2t2Rq (scaleRq2R2t (v' + (scaleR22Rq m)))) (v' + (scaleR22Rq m)).
+
+op cmq_expression (_A : Rq_mat) (s s': Rq_vec) (m : R2) : Rq =
+  let v' = v'_expression _A s s' in
+  v' + (scaleR22Rq m) + error_cmq _A s s' m.
+
+op m'_expression (_A : Rq_mat) (s s': Rq_vec) (m : R2) : R2 =
+  let v = v_expression _A s s' in
+  let cmq = cmq_expression _A s s' m in
+  scaleRq2R2 (v - cmq + (upscaleRq h2 (eq - ep))).
 
 
-lemma scaleZp2Zq_DM_big (F : int -> Zp) (r: int list) :
-  scaleZp2Zq (Rp.BasePoly.BigCf.BCA.big predT F r)
-  =
-  Rq.BasePoly.BigCf.BCA.big predT (scaleZp2Zq \o F) r.
-proof.
-elim: r => [| @/(\o) x l ih]. 
-+ by rewrite Rp.BasePoly.BigCf.BCA.big_nil Rq.BasePoly.BigCf.BCA.big_nil scaleZp2Zq0.
-+ rewrite Rp.BasePoly.BigCf.BCA.big_consT Rq.BasePoly.BigCf.BCA.big_consT /=.
-  by rewrite scaleZp2Zq_DM; congr.
-qed.
-
-lemma scaleRp2RqE (p : Rp) (i : int) : (scaleRp2Rq p).[i] = scaleZp2Zq p.[i].
-proof.
-case (i < 0) => [lt0_i | /lezNgt ge0_i]; 1: by rewrite !lt0_rcoeff 3:scaleZp2Zq0.
-case (i < n) => [ltn_i | /lezNgt gen_i]; last by rewrite !gered_rcoeff 3:scaleZp2Zq0.
-rewrite /scaleRp2Rq rcoeff_sum /=. 
-have ->: 
-  (fun (i0 : int) => (scaleZp2Zq p.[i0] ** exp Rq.iX i0).[i])
-  =
-  (fun (i0 : int) => scaleZp2Zq p.[i0] * (exp Rq.iX i0).[i]).
-+ by rewrite fun_ext /( == ) => x; apply Rq.rcoeffZ.
-rewrite (Rq.BasePoly.BigCf.BCA.bigD1 _ _ i) /=; 1, 2: by rewrite (mem_range, range_uniq).
-rewrite Rq.BasePoly.BigCf.BCA.big_seq_cond Rq.BasePoly.BigCf.BCA.big1 /= 2:Zq.ZModpRing.addr0
-        => [j [/mem_range rng_j @/predC1 ne_ji]|].
-+ by rewrite rcoeff_polyXn // (eq_sym i j) ne_ji /= Zq.ZModpRing.mulr0.
-+ by rewrite rcoeff_polyXn //= Zq.ZModpRing.mulr1.
-qed.
-
-lemma scaleRp2Rq_DM (p1 p2 : Rp) : scaleRp2Rq (p1 + p2) = scaleRp2Rq p1 + scaleRp2Rq p2.
-proof.
-by rewrite polyXnD1_eqP => i rng_i; rewrite rcoeffD !scaleRp2RqE rcoeffD scaleZp2Zq_DM.
-qed.
-
-lemma scaleRp2Rq_MA (p1 p2 : Rp) : scaleRp2Rq (p1 * p2) = scaleRp2Rq p1 * Rp2Rq p2.
-proof.
-rewrite polyXnD1_eqP => i rng_i; rewrite scaleRp2RqE !rcoeffM // scaleZp2Zq_DM_big /(\o). 
-rewrite !Rq.BasePoly.BigCf.BCA.big_seq &(Rq.BasePoly.BigCf.BCA.eq_bigr) /= => j /mem_range rng_j.
-by rewrite scaleZp2Zq_BM !scaleZp2Zq_MA -scaleRp2RqE -!Rp2RqE.
-qed.
-
-lemma scaleRp2Rq0 : scaleRp2Rq Rp.zeroXnD1 = Rq.zeroXnD1.
-proof. by rewrite polyXnD1_eqP => i rng_i; rewrite scaleRp2RqE !rcoeff0 scaleZp2Zq0. qed.
-
-lemma scaleRp2Rq_DM_big (F : int -> Rp) (r : int list) :
-  scaleRp2Rq (Mat_Rp.Big.BAdd.big predT F r)
-  =
-  Big.BAdd.big predT (scaleRp2Rq \o F) r.
-proof.
-elim: r => [| @/(\o) x l ih].
-+ by rewrite Mat_Rp.Big.BAdd.big_nil Big.BAdd.big_nil scaleRp2Rq0.
-+ rewrite Mat_Rp.Big.BAdd.big_consT Big.BAdd.big_consT /=.
-  by rewrite scaleRp2Rq_DM; congr.
-qed.
-
-lemma scaleRpv2RqvE (pv : Rp_vec) (i : int) : (scaleRpv2Rqv pv).[i] = scaleRp2Rq pv.[i].
-proof.
-rewrite /scaleRpv2Rqv /Mat_Rq.Vector."_.[_]" offunvK /vclamp.
-by case (0 <= i && i < l) => // rng_i; rewrite getv_out // scaleRp2Rq0.
-qed.
 
 (* 
-lemma Zq2Zp_DM_big (F : int -> Zq) (r : int list) :
-      Zq2Zp (Rq.BasePoly.BigCf.BCA.big predT F r)
-      =
-      BCA.big predT (Zq2Zp \o F) r.
-proof.
-elim: r; first by rewrite BCA.big_nil Rq.BasePoly.BigCf.BCA.big_nil Zq2Zp0.
-move => x l @/(\o) IH; rewrite BCA.big_cons Rq.BasePoly.BigCf.BCA.big_cons {1 4}/predT /=.
-by rewrite (Zq2Zp_DM (F x) (Rq.BasePoly.BigCf.BCA.big predT F l)); congr.
-qed.
+bq <- scaleRpv2Rqv b;
+b <- scaleRqv2Rpv (_A *^ s + h)
+==>
+bq <- scaleRpv2Rqv (scaleRqv2Rpv (_A *^ s + h))
+
+
+bq' <- scaleRpv2Rqv b';
+b' <- scaleRqv2Rpv ((trmx _A) *^ s' + h);
+==>
+bq' <- scaleRpv2Rqv (scaleRqv2Rpv ((trmx _A) *^ s' + h));
+
+
+cmq <- scaleR2t2Rq cm;
+cm <- scaleRq2R2t (v' + (scaleR22Rq m_dec));
+==>
+cmq <- scaleR2t2Rq (scaleRq2R2t (v' + (scaleR22Rq m_dec)));
+
+m' <- scaleRq2R2 (v - cmq + (upscaleRq h2 (eq - ep)))   
+v <- (dotp bq' s) + (upscaleRq h1 (eq - ep))
+
+
 *)
-
-lemma Zp2Zq0 : Zp2Zq Zp.zero = Zq.zero.
-proof. by rewrite /Zp2Zq -asintK !zeroE. qed.
-
-lemma Zq2Zp_Zp2Zq_small_inv (z : Zq) : asint z < p => Zp2Zq (Zq2Zp z) = z.
-proof.
-move => ltp_z; by rewrite /Zq2Zp /Zp2Zq -{2}asintK inzmodK pmod_small 2?(ge0_asint, ltp_z).
-qed.
-
-(*
-lemma Zp2Zq_DM : morphism_2 Zp2Zq Zp.( + ) Zq.( + ).
-proof.
-move => x y. rewrite /Zp2Zq addE -inzmodD -eq_inzmod.
-qed.
-
-lemma Zp2Zq_DM_big (F : int -> Zp) (r : int list) :
-      Zp2Zq (Rp.BasePoly.BigCf.BCA.big predT F r)
-      =
-      Rq.BasePoly.BigCf.BCA.big predT (Zp2Zq \o F) r.
-proof.
-elim: r; first by rewrite Rp.BasePoly.BigCf.BCA.big_nil Rq.BasePoly.BigCf.BCA.big_nil Zp2Zq0.
-move => x l @/(\o) ih; rewrite  Rp.BasePoly.BigCf.BCA.big_consT Rq.BasePoly.BigCf.BCA.big_consT.
-by rewrite Zp2Zq_DM; congr.
-qed.
-*)
-
-lemma Rq2Rp_Rp2Rq_small_inv (p : Rq) : p \in dsmallRq => Rp2Rq (Rq2Rp p) = p.
-proof.
-move /supp_dsmallRq => val_coeff; rewrite polyXnD1_eqP => i rngi.
-by rewrite rcoeffZ_sum //= rcoeffZ_sum //= Zq2Zp_Zp2Zq_small_inv 1:(val_coeff i).
-qed.
-
-(* dotp (q/p * b) s + (q/p * h1)  =  q / p * (dotp b s + h1) *)
-(* dotp (q/p * b) s = q/p * (dotp b s) *) 
-lemma scaleRp2Rq_DotDM (b : Rp_vec) (s : Rq_vec) : 
-  s \in dsmallRq_vec => dotp (scaleRpv2Rqv b) s = scaleRp2Rq (dotp b (Rqv2Rpv s)).
-proof.
-move /supp_dsmallRq_vec => val_coeff; rewrite /dotp scaleRp2Rq_DM_big /(\o).
-rewrite !Big.BAdd.big_seq &(Big.BAdd.eq_bigr) /= => i /mem_range rng_i.
-by rewrite Rqv2RpvE scaleRp2Rq_MA scaleRpv2RqvE Rq2Rp_Rp2Rq_small_inv 1:val_coeff.
-qed.
-
-lemma scaleRq_h1 : scaleRq h1 (eq - ep) = scaleRp2Rq (Rq2Rp h1).
-proof.
-rewrite polyXnD1_eqP => i rng_i.
-rewrite rcoeffZ_sum //= eq_sym rcoeffZ_sum //=. 
-rewrite /Rq2Rp. rewrite (Rp.rcoeffZ_sum (fun (i0 : int) => Zq2Zp h1.[i0])) //=.
-rewrite rcoeffZ_sum //=. rewrite /scaleZp2Zq /scaleZq /Zq2Zp -eq_inzmod.
-rewrite !inzmodK. rewrite /q /p modz_dvd_pow. smt(ge2_ep geep1_eq).
-have tt: 2 ^ (eq - ep - 1) < 2 ^ ep. admit.
-rewrite !(pmod_small (2 ^ (eq - ep - 1))). admit. admit.
-trivial.
-qed. 
-
-lemma scaleRq_h2 : scaleRq h2 (eq - ep) = scaleRp2Rq (Rq2Rp h2).
-proof.
-rewrite polyXnD1_eqP => i rng_i.
-rewrite rcoeffZ_sum //= eq_sym rcoeffZ_sum //=. 
-rewrite /Rq2Rp. rewrite (Rp.rcoeffZ_sum (fun (i0 : int) => Zq2Zp h2.[i0])) //=.
-rewrite rcoeffZ_sum //=. rewrite /scaleZp2Zq /scaleZq /Zq2Zp -eq_inzmod.
-rewrite !inzmodK.  rewrite /q /p modz_dvd_pow. smt(ge2_ep geep1_eq).
-have tt: (2 ^ (ep - 2) - 2 ^ (ep - et - 2)) < 2 ^ ep. admit.
-rewrite !(pmod_small ((2 ^ (ep - 2) - 2 ^ (ep - et - 2)))). admit. admit.
-trivial.
-qed.
+op error_expression () : 
 
 
-
-lemma scaleRp2R2_DM (p1 p2 : Rp) : 
-  ((forall (i : int), 0 <= i < n =>  2 ^ (ep - 1) %| Zp.asint p1.[i]) \/  
-  (forall (i : int), 0 <= i < n =>  2 ^ (ep - 1) %| Zp.asint p2.[i])) =>
-  scaleRp2R2 (p1 + p2) = scaleRp2R2 p1 + scaleRp2R2 p2.
-proof.
-case => [divz1 | divz2]; rewrite /scaleRp2R2 eq_sym -BigR2.XnD1CA.big_split /=;
-    rewrite !BigR2.XnD1CA.big_seq &(BigR2.XnD1CA.eq_bigr) /= => i /mem_range rng_i;
-    rewrite -scaleDl eq_sym rcoeffD scaleZp2Z2_DM ?(divz1, divz2) //.
-qed.
-
-lemma scaleRq2R2_DM (p1 p2 : Rq) : 
-  ((forall (i : int), 0 <= i < n =>  2 ^ (eq - 1) %| Zq.asint p1.[i]) \/  
-  (forall (i : int), 0 <= i < n =>  2 ^ (eq - 1) %| Zq.asint p2.[i])) =>
-  scaleRq2R2 (p1 + p2) = scaleRq2R2 p1 + scaleRq2R2 p2.
-proof.
-case => [divz1 | divz2]; rewrite /scaleRq2R2 eq_sym -BigR2.XnD1CA.big_split /=;
-    rewrite !BigR2.XnD1CA.big_seq &(BigR2.XnD1CA.eq_bigr) /= => i /mem_range rng_i;
-    rewrite -scaleDl eq_sym rcoeffD scaleZq2Z2_DM ?(divz1, divz2) //.
-qed.
-
-lemma scaleR2t2Rq_shldec_c (c : R2t) :
-  scaleR2t2Rq c = scaleRp2Rq (shl_dec c).
-proof.
-   rewrite /scaleR2t2Rq /scaleRp2Rq.
-rewrite polyXnD1_eqP => i rngi.
-rewrite !rcoeffZ_sum //=.
-rewrite /shl_dec rcoeffZ_sum //=.
-rewrite /scaleZp2Zq /upscale /shl inzmodK.
-rewrite /scaleZ2t2Zq /upscale /shl -eq_inzmod.
-rewrite /p /q modz_pow2_mul. smt(ge2_ep geep1_eq).
-rewrite mulzA.
-rewrite -exprD_nneg; 1, 2: smt(geet2_ep geep1_eq). do 4! congr. by ring.
-qed. 
-
-lemma scaleZp2Zq_N (z : Zp) : scaleZp2Zq (- z) = - scaleZp2Zq z.
-proof.
-rewrite /scaleZp2Zq /upscale /shl -eq_inzmod !inzmodK /p /q modz_pow2_mul; 1: smt(ge2_ep geep1_eq).
-by rewrite modzNm mulNr.
-qed.
-
-lemma scaleRp2Rq_N (p : Rp): scaleRp2Rq (- p) = - scaleRp2Rq p.
-proof.
-rewrite /scaleRp2Rq polyXnD1_sumN /= polyXnD1_eqP => i rng_i.
-rewrite rcoeffZ_sum //; pose F k := - scaleZp2Zq p.[k].
-have -> /=:
-  ((BigRq.XnD1CA.bigi predT (fun (i0 : int) => - scaleZp2Zq p.[i0] ** exp Rq.iX i0) 0 n))
-  = 
-  ((BigRq.XnD1CA.bigi predT (fun (i0 : int) => F i0 ** exp Rq.iX i0) 0 n)).
-+ by rewrite 2!BigRq.XnD1CA.big_seq &(BigRq.XnD1CA.eq_bigr) /= => *; rewrite -scaleN.
-by rewrite rcoeffZ_sum // /F -rcoeffN scaleZp2Zq_N.
-qed.
-
-lemma scaleRp2Rq_BM (p1 p2 : Rp) : scaleRp2Rq (p1 - p2) = scaleRp2Rq p1 - scaleRp2Rq p2.
-proof. by rewrite scaleRp2Rq_DM -Rq.ComRing.addrC scaleRp2Rq_N Rq.ComRing.addrC. qed.
-
-lemma scaleZp2Zq2Z2_comp (z : Zp) : scaleZq2Z2 (scaleZp2Zq z) = scaleZp2Z2 z.
-proof.
-rewrite /scaleZq2Z2 /scaleZp2Zq /scaleZp2Z2 /downscale /upscale /shr /shl -eq_inzmod !inzmodK /p /q.
-rewrite modz_pow2_div 1:?(mulr_ge0, ge0_asint, expr_ge0); 1, 2: smt(geep1_eq ge3_eq).
-have ->: 2 ^ (eq - 1) = 2 ^ (ep - 1) * 2 ^ (eq - ep).
-+ by rewrite -exprD_nneg; 1, 2: smt(ge2_ep geep1_eq); congr; ring.
-by rewrite divzMpr 1:expr_gt0 2:opprD 2:addrA //= expr1 modz_mod.
-qed.
-
-module Saber_PKE_Scheme_Rq : Scheme = {
-   proc kg() : pkey * skey = {
-      var sd: seed;
-      var _A: Rq_mat;
-      var s: Rq_vec;
-      var b: Rp_vec;
-      
-      sd <$ dseed;
-      _A <- gen sd;
-      s <$ dsmallRq_vec;
-      b <- scaleRqv2Rpv (_A *^ s + h);
-      
-      return (pk_encode_s (sd, b), sk_encode_s s);
-   }
-
-   proc enc(pk: pkey, m: plaintext) : ciphertext = {
-      var pk_dec: seed * Rp_vec;
-      var m_dec: R2;
-
-      var sd: seed;
-      var _A: Rq_mat;
-      var s': Rq_vec;
-      var b, b': Rp_vec;
-      var bq: Rq_vec;
-      var v': Rq;
-      var cm: R2t;
-      
-      m_dec <- m_decode m;
-      pk_dec <- pk_decode_s pk;
-      sd <- pk_dec.`1;
-      b <- pk_dec.`2;
-      _A <- gen sd;
-      s' <$ dsmallRq_vec;
-      b' <- scaleRqv2Rpv ((trmx _A) *^ s' + h);
-      bq <- scaleRpv2Rqv b;
-      v' <- (dotp bq s') + (scaleRq h1 (eq - ep));
-      cm <- scaleRq2R2t (v' + (scaleR22Rq m_dec));
-      
-      return c_encode_s (cm, b');
-   }
-
-   proc dec(sk: skey, c: ciphertext) : plaintext option = {
-      var c_dec: R2t * Rp_vec;
-      var cm: R2t;
-      var cmq: Rq;
-      var b': Rp_vec;
-      var bq': Rq_vec;
-      var v: Rq;
-      var s: Rq_vec;
-      var m': R2;
-
-      c_dec <- c_decode_s c;
-      s <- sk_decode_s sk;
-      cm <- c_dec.`1;
-      cmq <- scaleR2t2Rq cm;
-      b' <- c_dec.`2;
-      bq' <- scaleRpv2Rqv b';
-      
-      v <- (dotp bq' s) + (scaleRq h1 (eq - ep));
-      m' <- scaleRq2R2 (v  - cmq + (scaleRq h2 (eq - ep)));
-      
-      return Some (m_encode m');
-   }
-}.
-
-
-lemma eq_kg: equiv[Saber_PKE_Scheme.kg ~ Saber_PKE_Scheme_Rq.kg : true ==> ={res}].
-proof.
-by proc; sim.
-qed.
-
-lemma eq_enc: equiv[Saber_PKE_Scheme.enc ~ Saber_PKE_Scheme_Rq.enc : ={pk, m} ==> ={res}].
-proof.
-proc.
-auto; progress. 
-congr; rewrite &(pw_eq) //.
-rewrite scaleRp2R2t_DM 2: scaleRq2R2t_DM; 1, 2: right => i rng_i.
-+ rewrite rcoeffZ_sum //= inzmodK /shl.
-  case (asint (m_decode m{2}).[i] = 0) => [-> /= | neq0_m].
-  - by apply dvdz0.
-  - have -> /=:  (Z2.asint (m_decode m{2}).[i]) = 1. admit.
-    rewrite pmod_small. admit.
-    by apply dvdz_exp2l; smt(ge0_et geet2_ep). 
-+ rewrite rcoeffZ_sum //= inzmodK /upscale /shl. 
-  case (asint (m_decode m{2}).[i] = 0) => [-> /= | neq0_m].
-  - by apply dvdz0.
-  - have -> /=:  (Z2.asint (m_decode m{2}).[i]) = 1. admit.
-    rewrite pmod_small. admit.
-    by apply dvdz_exp2l; smt(ge0_et geet2_ep geep1_eq). 
-congr; last first.
-+ rewrite polyXnD1_eqP /shl_enc /scaleR22Rq => i rngi.
-  rewrite !rcoeffZ_sum //= !rcoeffZ_sum //=.
-  rewrite eq_sym /scaleZq2Z2t /scaleZ22Zq inzmodK.
-  rewrite eq_sym /scaleZp2Z2t inzmodK -eq_inzmod.
-  rewrite /upscale /shl (pmod_small _ p) 2:(pmod_small _ q). admit. admit.
-  rewrite /downscale /shr (_ : 2 ^ (ep - 1) = 2 ^ (ep - (et + 1)) * 2 ^ et).
-  rewrite -exprD_nneg; 1, 2: smt(geet2_ep ge0_et). congr. ring.
-  rewrite (mulzC _ (2 ^ et)) -mulzA mulzK. admit.
-  rewrite (_ : 2 ^ (eq - 1) = 2 ^ (eq - (et + 1)) * 2 ^ et).
-  rewrite -exprD_nneg; 1, 2: smt(geet2_ep geep1_eq ge0_et).
-  congr. ring.
-  rewrite eq_sym (mulzC _ (2 ^ et)) -mulzA mulzK. admit. trivial.
-+ rewrite eq_sym scaleRp2Rq_DotDM // scaleRq_h1 -scaleRp2Rq_DM.
-  rewrite polyXnD1_eqP => i rng_i.
-  rewrite !rcoeffZ_sum //= rcoeffZ_sum //=. 
-  rewrite /scaleZq2Z2t /scaleZp2Zq !inzmodK.
-  rewrite /scaleZp2Z2t -eq_inzmod /downscale /upscale /shr /shl /q /t -exprS 1:ge0_et.
-  rewrite modz_pow2_div. admit. smt(ge0_et geet2_ep geep1_eq).
-  rewrite (_ : 2 ^ (eq - (eq - (et + 1))) = 2 ^ (et + 1)) 2:modz_mod. congr; ring.
-  rewrite (_ : 2 ^ (eq - (et + 1)) = 2 ^ (eq - ep) * 2 ^ (ep - (et + 1))).
-  rewrite -exprD_nneg; 1,2: smt(geet2_ep geep1_eq). congr; ring.
-  rewrite -(mulzC (2 ^ (ep - (et + 1)))) divzMpr. admit.
-  trivial.
-qed.
-
-lemma eq_dec: equiv[Saber_PKE_Scheme.dec ~ Saber_PKE_Scheme_Rq.dec : 
-  ={sk, c} /\ 
-  sk_decode_s sk{1} \in dsmallRq_vec /\
-  sk_decode_s sk{2} \in dsmallRq_vec
-  ==> 
-  ={res}].
-proof.
-proc.
-auto; progress.
-congr.
-rewrite scaleRp2Rq_DotDM //.
-rewrite scaleRq_h1 scaleRq_h2 scaleR2t2Rq_shldec_c.
-rewrite Rq.ComRing.addrC.
-rewrite Rp.ComRing.addrC.
-rewrite Rq.ComRing.addrA.
-rewrite Rp.ComRing.addrA.
-rewrite -scaleRp2Rq_DM.
-rewrite -scaleRp2Rq_DM.
-rewrite -scaleRp2Rq_BM.
-rewrite polyXnD1_eqP => i rng_i; rewrite eq_sym /scaleRq2R2 !rcoeffZ_sum //= rcoeffZ_sum //=.
-rewrite scaleZp2Zq2Z2_comp. trivial.
-qed.
-
-(* TODO:
-- Change definitions of regular scheme regarding encoding/decoding such that
-  we can use the types of the artifacts in above proof (i.e., dont use encoding/decoding
-  when unnecessary, and when necesarry, a seperate one for regular scheme with concrete typing).
-- Remove all admits.
-- Define subtype for secret key (only taking values currently in dsmallRq_vec), and have that be the domain and range of s_encode and s_decode, respectively.
-- Clean up.
-*)
-*)
